refactor: Move to one file and rename

PhysLean/StringTheory/FTheory/SU5U1/Charges/Yukawa/Elems.lean
@@ -11,6 +11,11 @@ import Mathlib.Tactic.FinCases
 
 # Charges which are not phenoconstrained and do not regenerate dangerous couplings with Yukawas
 
+In this module we give a multiset of `ℤ`-valued charges which have values allowed
+by a `CodimensionOneConfig`, `I`, which permit a top Yukawa coupling,
+are not phenomenologically constrained, and do not regenerate dangerous couplings
+with one insertion of a Yuakawa coupling.
+
 
 -/
 namespace FTheory
@@ -25,30 +30,241 @@ open CodimensionOneConfig
 open Tree
 open PhysLean
 
-/-- For a given `I : CodimensionOneConfig` the tree of charges containing all
-  charges which are not phenomenlogically constrained, and which permit a top
-  Yukawa coupling. Unlike `nonPhenoConstrainedCharges`, these trees are calculated
-  and therefore not good when using `decide` etc.
--/
-def nonPhenoConstrainedChargesExt (I : CodimensionOneConfig) :
-    Multiset (Charges ℤ) :=
-  let completionTopYukawa := (((minimallyAllowsTermsOfFinset I.allowedBarFiveCharges
-      I.allowedTenCharges topYukawa).bind
-    (completions I.allowedBarFiveCharges I.allowedTenCharges)).dedup.filter
-    (fun x => ¬ IsPhenoConstrained x))
-  let addOneTopYukawa := (((completionTopYukawa).bind (fun x =>
-    (minimalSuperSet I.allowedBarFiveCharges I.allowedTenCharges x).val)).dedup.filter
-    (fun x => ¬ IsPhenoConstrained x))
-  let addTwoTopYukawa := (((addOneTopYukawa).bind (fun x =>
-    (minimalSuperSet I.allowedBarFiveCharges I.allowedTenCharges x).val)).dedup.filter
-    (fun x => ¬ IsPhenoConstrained x))
-  let addThreeTopYukawa := (((addTwoTopYukawa).bind (fun x =>
-    (minimalSuperSet I.allowedBarFiveCharges I.allowedTenCharges x).val)).dedup.filter
-    (fun x => ¬ IsPhenoConstrained x))
-  ((completionTopYukawa + addOneTopYukawa +
-    addTwoTopYukawa + addThreeTopYukawa).filter fun x => ¬ YukawaGeneratesDangerousAtLevel x 1)
+/-!
 
-private def nonPhenoConstrainedChargesSame : Multiset (Charges ℤ) :=
+## Viable completions
+
+-/
+
+
+/--
+The tree of charges which contains all `completions` of
+charges which minimally allow the top Yukawa,
+which are not pheno-constrained.
+
+This can be constructed via
+
+#eval FourTree.fromMultiset <|
+    ((minimallyAllowsTermsOfFinset same.allowedBarFiveCharges
+        same.allowedTenCharges topYukawa).bind <|
+      completions same.allowedBarFiveCharges same.allowedTenCharges).dedup.filter
+    fun x => ¬ IsPhenoConstrained x
+-/
+private def viableCompletions (I : CodimensionOneConfig) : Multiset (Charges ℤ) :=
+  match I with
+  | same => {(some (-2), some (-3), {2}, {-3, 0}), (some (-1), some (-3), {1}, {-3, 0}),
+    (some 1, some (-3), {-1}, {-3, 0}), (some 1, some (-3), {2}, {-3, 0}),
+    (some 2, some (-3), {-2}, {-3, 0}), (some 2, some (-3), {1}, {-3, 0}),
+    (some (-3), some (-2), {0}, {-1}), (some (-3), some (-2), {1}, {-1}),
+    (some (-3), some (-2), {2}, {-1}), (some (-1), some (-2), {0}, {-1}),
+    (some (-1), some (-2), {1}, {-1}), (some (-1), some (-2), {2}, {-1}),
+    (some 0, some (-2), {-3}, {-1}), (some 0, some (-2), {-1}, {-1}),
+    (some 0, some (-2), {1}, {-1}), (some 0, some (-2), {2}, {-1}),
+    (some 1, some (-2), {-3}, {-1}), (some 1, some (-2), {-1}, {-1}),
+    (some 1, some (-2), {0}, {-1}), (some 1, some (-2), {2}, {-1}),
+    (some 2, some (-2), {-3}, {-1}), (some 2, some (-2), {-1}, {-1}),
+    (some 2, some (-2), {0}, {-1}), (some 2, some (-2), {1}, {-1}),
+    (some (-3), some (-2), {3}, {-2, 0}), (some (-1), some (-2), {3}, {-2, 0}),
+    (some 3, some (-2), {-3}, {-2, 0}), (some (-1), some (-2), {0}, {-3, 1}),
+    (some 0, some (-2), {-1}, {-3, 1}), (some 0, some (-2), {3}, {-3, 1}),
+    (some 3, some (-2), {0}, {-3, 1}), (some (-2), some 0, {-1}, {-3, 3}),
+    (some (-2), some 0, {1}, {-3, 3}), (some (-1), some 0, {-2}, {-3, 3}),
+    (some (-1), some 0, {2}, {-3, 3}), (some 1, some 0, {-2}, {-3, 3}),
+    (some 1, some 0, {2}, {-3, 3}), (some 2, some 0, {-1}, {-3, 3}),
+    (some 2, some 0, {1}, {-3, 3}), (some (-2), some 2, {-1}, {1}),
+    (some (-2), some 2, {0}, {1}), (some (-2), some 2, {1}, {1}),
+    (some (-2), some 2, {3}, {1}), (some (-1), some 2, {-2}, {1}),
+    (some (-1), some 2, {0}, {1}), (some (-1), some 2, {1}, {1}),
+    (some (-1), some 2, {3}, {1}), (some 0, some 2, {-2}, {1}),
+    (some 0, some 2, {-1}, {1}), (some 0, some 2, {1}, {1}),
+    (some 0, some 2, {3}, {1}), (some 1, some 2, {-2}, {1}),
+    (some 1, some 2, {-1}, {1}), (some 1, some 2, {0}, {1}),
+    (some 3, some 2, {-2}, {1}), (some 3, some 2, {-1}, {1}),
+    (some 3, some 2, {0}, {1}), (some (-3), some 2, {3}, {0, 2}),
+    (some 1, some 2, {-3}, {0, 2}), (some 3, some 2, {-3}, {0, 2}),
+    (some (-3), some 2, {0}, {-1, 3}), (some 0, some 2, {-3}, {-1, 3}),
+    (some 0, some 2, {1}, {-1, 3}), (some 1, some 2, {0}, {-1, 3}),
+    (some (-2), some 3, {-1}, {0, 3}), (some (-2), some 3, {2}, {0, 3}),
+    (some (-1), some 3, {-2}, {0, 3}), (some (-1), some 3, {1}, {0, 3}),
+    (some 1, some 3, {-1}, {0, 3}), (some 2, some 3, {-2}, {0, 3})}
+  | nearestNeighbor => {(some (-9), some (-14), {-4}, {-7}), (some (-9), some (-14), {1}, {-7}),
+    (some (-9), some (-14), {6}, {-7}), (some (-9), some (-14), {11}, {-7}),
+    (some (-4), some (-14), {-9}, {-7}), (some (-4), some (-14), {1}, {-7}),
+    (some (-4), some (-14), {6}, {-7}), (some (-4), some (-14), {11}, {-7}),
+    (some 1, some (-14), {-9}, {-7}), (some 1, some (-14), {-4}, {-7}),
+    (some 1, some (-14), {6}, {-7}), (some 1, some (-14), {11}, {-7}),
+    (some 6, some (-14), {-9}, {-7}), (some 6, some (-14), {-4}, {-7}),
+    (some 6, some (-14), {1}, {-7}), (some 6, some (-14), {11}, {-7}),
+    (some 11, some (-14), {-9}, {-7}), (some 11, some (-14), {-4}, {-7}),
+    (some 11, some (-14), {1}, {-7}), (some 11, some (-14), {6}, {-7}),
+    (some 11, some (-14), {-9}, {-12, -2}), (some 1, some (-9), {11}, {-12, 3}),
+    (some 11, some (-9), {1}, {-12, 3}), (some (-14), some (-4), {-9}, {-2}),
+    (some (-14), some (-4), {11}, {-2}), (some (-9), some (-4), {-14}, {-2}),
+    (some (-9), some (-4), {11}, {-2}), (some 1, some (-4), {-14}, {-2}),
+    (some 1, some (-4), {11}, {-2}), (some 11, some (-4), {-14}, {-2}),
+    (some 11, some (-4), {-9}, {-2}), (some (-9), some 1, {-4}, {-12, 13}),
+    (some (-4), some 1, {-9}, {-12, 13}), (some 6, some 1, {-9}, {-12, 13}),
+    (some (-14), some 6, {-4}, {3}), (some (-14), some 6, {1}, {3}),
+    (some (-14), some 6, {11}, {3}), (some (-4), some 6, {-14}, {3}),
+    (some (-4), some 6, {1}, {3}), (some (-4), some 6, {11}, {3}),
+    (some 1, some 6, {-14}, {3}), (some 1, some 6, {-4}, {3}),
+    (some 11, some 6, {-14}, {3}), (some 11, some 6, {-4}, {3}),
+    (some (-9), some 6, {-4}, {-7, 13}), (some (-4), some 6, {-9}, {-7, 13}),
+    (some (-4), some 6, {11}, {-7, 13}), (some 11, some 6, {-4}, {-7, 13})}
+  | nextToNearestNeighbor => {(some (-13), some (-8), {7}, {-4}),
+    (some (-3), some (-8), {7}, {-4}), (some 2, some (-8), {-13}, {-4}),
+    (some 2, some (-8), {-3}, {-4}), (some 2, some (-8), {7}, {-4}),
+    (some 7, some (-8), {-13}, {-4}), (some 7, some (-8), {-3}, {-4}),
+    (some (-13), some 2, {-8}, {1}), (some (-13), some 2, {7}, {1}),
+    (some (-13), some 2, {12}, {1}), (some (-8), some 2, {-13}, {1}),
+    (some (-8), some 2, {7}, {1}), (some 7, some 2, {-13}, {1}),
+    (some 7, some 2, {-8}, {1}), (some 7, some 2, {12}, {1}),
+    (some 12, some 2, {-13}, {1}), (some 12, some 2, {7}, {1}),
+    (some (-8), some 2, {-3}, {-9, 11}), (some (-3), some 2, {-8}, {-9, 11}),
+    (some (-3), some 2, {12}, {-9, 11}), (some 12, some 2, {-3}, {-9, 11}),
+    (some (-13), some 12, {-8}, {6}), (some (-13), some 12, {2}, {6}),
+    (some (-13), some 12, {7}, {6}), (some (-8), some 12, {-13}, {6}),
+    (some (-8), some 12, {2}, {6}), (some (-8), some 12, {7}, {6}),
+    (some (-3), some 12, {-13}, {6}), (some (-3), some 12, {-8}, {6}),
+    (some (-3), some 12, {2}, {6}), (some (-3), some 12, {7}, {6}),
+    (some 2, some 12, {-13}, {6}), (some 2, some 12, {-8}, {6}),
+    (some 2, some 12, {7}, {6}), (some 7, some 12, {-13}, {6}),
+    (some 7, some 12, {-8}, {6}), (some 7, some 12, {2}, {6})}
+
+lemma viableCompletions_card (I : CodimensionOneConfig) :
+    (viableCompletions I).card = if I = same then 70 else
+      if I = nearestNeighbor then 48 else 37 := by
+  cases I <;> rfl
+
+lemma viableCompletions_nodup (I : CodimensionOneConfig) :
+    (viableCompletions I).Nodup := by
+  cases I <;> decide
+
+/-!
+
+## Viable completions
+
+We now prove that `viableCompletions I` contains all completions of
+charges which minimally allow the top Yukawa, which are not
+phenomenologically constrained, and which do not regenerate dangerous couplings
+with one insertion of a Yukawa coupling.
+
+This is broken up into a series of lemmas, but the main result is:
+`viableCompletions_complete`.
+
+-/
+
+lemma viableCompletions_complete_of_same :
+    ∀ x ∈ (minimallyAllowsTermsOfFinset CodimensionOneConfig.same.allowedBarFiveCharges
+      CodimensionOneConfig.same.allowedTenCharges topYukawa),
+    ¬ x.IsPhenoConstrained →
+    ∀ y ∈ completions same.allowedBarFiveCharges same.allowedTenCharges x, ¬ y.IsPhenoConstrained
+    ∧ ¬ y.YukawaGeneratesDangerousAtLevel 1
+    → y ∈ viableCompletions .same := by
+  decide
+
+
+lemma viableCompletions_complete_of_nearestNeighbor :
+    ∀ x ∈ (minimallyAllowsTermsOfFinset
+      CodimensionOneConfig.nearestNeighbor.allowedBarFiveCharges
+      CodimensionOneConfig.nearestNeighbor.allowedTenCharges topYukawa),
+    ¬ x.IsPhenoConstrained →
+    ∀ y ∈ completions nearestNeighbor.allowedBarFiveCharges
+      nearestNeighbor.allowedTenCharges x, ¬ y.IsPhenoConstrained
+      ∧ ¬ y.YukawaGeneratesDangerousAtLevel 1
+    → y ∈ viableCompletions .nearestNeighbor := by
+  decide
+
+lemma viableCompletions_complete_of_nextToNearestNeighbor :
+    ∀ x ∈ (minimallyAllowsTermsOfFinset
+      CodimensionOneConfig.nextToNearestNeighbor.allowedBarFiveCharges
+      CodimensionOneConfig.nextToNearestNeighbor.allowedTenCharges topYukawa),
+    ¬ x.IsPhenoConstrained →
+    ∀ y ∈ completions nextToNearestNeighbor.allowedBarFiveCharges
+      nextToNearestNeighbor.allowedTenCharges x, ¬ y.IsPhenoConstrained
+      ∧ ¬ y.YukawaGeneratesDangerousAtLevel 1
+    → y ∈ viableCompletions .nextToNearestNeighbor := by
+  decide
+
+lemma viableCompletions_complete {I : CodimensionOneConfig} (x : Charges)
+    (hx : x ∈ (minimallyAllowsTermsOfFinset I.allowedBarFiveCharges
+      I.allowedTenCharges topYukawa))
+    (hPheno : ¬ x.IsPhenoConstrained) :
+    ∀ y ∈ completions I.allowedBarFiveCharges I.allowedTenCharges x, ¬ y.IsPhenoConstrained
+    ∧ ¬ y.YukawaGeneratesDangerousAtLevel 1
+    → y ∈ viableCompletions I := by
+  cases I
+  case same => exact viableCompletions_complete_of_same x hx hPheno
+  case nearestNeighbor => exact viableCompletions_complete_of_nearestNeighbor x hx hPheno
+  case nextToNearestNeighbor => exact
+    viableCompletions_complete_of_nextToNearestNeighbor x hx hPheno
+
+/-!
+
+## Existence of a subset in `viableCompletions`
+-/
+
+set_option maxRecDepth 2000 in
+/-- Every charge `x : Charges` with values determined by an `I : CodimensionOneConfig`,
+  which is not phenomenologically constrained, permits the top Yukawa, and
+  does not regenerate danergours couplings with the Yukawa terms,
+  has a subset which is contained within `viableCompletions I`.  -/
+lemma exists_subset_viableCompletions_of_not_isPhenoConstrained {x : Charges}
+    (hx : ¬ x.IsPhenoConstrained ∧ ¬ x.YukawaGeneratesDangerousAtLevel 1)
+    (htopYukawa : AllowsTerm x topYukawa)
+    (hsub : x ∈ ofFinset I.allowedBarFiveCharges I.allowedTenCharges)
+    (hcomplete : IsComplete x) : ∃ (y : Charges), y ∈ viableCompletions I ∧ y ⊆ x := by
+  have hIrreducible :
+        ∃ y ∈ (minimallyAllowsTermsOfFinset I.allowedBarFiveCharges
+        I.allowedTenCharges topYukawa), y ⊆ x := by
+      rw [allowsTerm_iff_subset_minimallyAllowsTerm] at htopYukawa
+      obtain ⟨y, hPower, hIrre⟩ := htopYukawa
+      use y
+      constructor
+      · rw [← minimallyAllowsTerm_iff_mem_minimallyAllowsTermOfFinset]
+        · exact hIrre
+        · simp at hPower
+          exact mem_ofFinset_antitone I.allowedBarFiveCharges I.allowedTenCharges hPower hsub
+      · simpa using hPower
+  obtain ⟨y, hyMem, hysubsetx⟩ := hIrreducible
+  obtain ⟨z, hz1, hz2⟩ := exist_completions_subset_of_complete
+    I.allowedBarFiveCharges I.allowedTenCharges y x hysubsetx hsub hcomplete
+  use z
+  constructor
+  · refine viableCompletions_complete y hyMem ?_ z hz1 ?_
+    · by_contra hn
+      have h' := isPhenoConstrained_mono hysubsetx hn
+      simp_all
+    · apply And.intro
+      · by_contra hn
+        have h' := isPhenoConstrained_mono hz2 hn
+        simp_all
+      · by_contra hn
+        have h' := yukawaGeneratesDangerousAtLevel_of_subset hz2 hn
+        simp_all
+  · simp_all
+/-!
+
+## The multisets of viable charges.
+
+-/
+
+TODO "JGVOQ" "Make the result `viableChargesExt` a safe definition."
+
+unsafe def viableChargesExt (I : CodimensionOneConfig) :
+    Multiset (Charges ℤ) :=
+    (aux (viableCompletions I) (viableCompletions I)).dedup
+where
+  aux : Multiset (Charges ℤ) →  Multiset (Charges ℤ) →  Multiset (Charges ℤ) :=
+    fun all add  =>
+      if add = ∅ then all else
+      let s := add.bind fun x =>
+         (minimalSuperSet I.allowedBarFiveCharges I.allowedTenCharges x).val
+      let s2 := s.filter fun y => y ∉ all ∧
+        ¬ IsPhenoConstrained y ∧ ¬ YukawaGeneratesDangerousAtLevel y 1
+      aux (all + s2) s2
+
+private def viableChargesSame : Multiset (Charges ℤ) :=
    {(some (-2), some (-3), {2}, {-3, 0}), (some (-1), some (-3), {1}, {-3, 0}),
     (some 1, some (-3), {-1}, {-3, 0}), (some 1, some (-3), {2}, {-3, 0}),
     (some 2, some (-3), {-2}, {-3, 0}), (some 2, some (-3), {1}, {-3, 0}),
@@ -101,7 +317,7 @@ private def nonPhenoConstrainedChargesSame : Multiset (Charges ℤ) :=
     (some (-2), some 3, {-1, 2}, {0, 3}), (some (-1), some 3, {-2, 1}, {0, 3}),
     (some 0, some (-2), {-3, 1}, {3, -1}), (some 0, some 2, {-1, 3}, {-3, 1})}
 
-private def nonPhenoConstrainedChargesNN : Multiset (Charges ℤ) :=
+private def viableChargesNN : Multiset (Charges ℤ) :=
   {(some (-9), some (-14), {-4}, {-7}), (some (-9), some (-14), {1}, {-7}),
     (some (-9), some (-14), {6}, {-7}), (some (-9), some (-14), {11}, {-7}),
     (some (-4), some (-14), {-9}, {-7}), (some (-4), some (-14), {1}, {-7}),
@@ -139,7 +355,7 @@ private def nonPhenoConstrainedChargesNN : Multiset (Charges ℤ) :=
     (some 11, some 6, {-14, -4}, {3}), (some (-4), some 6, {-9, 11}, {-7, 13}),
     (some (-4), some (-14), {-9, 11}, {13, -7})}
 
-private def nonPhenoConstrainedChargesNtoNN : Multiset (Charges ℤ) :=
+private def viableChargesNtoNN : Multiset (Charges ℤ) :=
   {(some (-13), some (-8), {7}, {-4}), (some (-3), some (-8), {7}, {-4}),
     (some 2, some (-8), {-13}, {-4}), (some 2, some (-8), {-3}, {-4}),
     (some 2, some (-8), {7}, {-4}), (some 7, some (-8), {-13}, {-4}),
@@ -173,10 +389,10 @@ private def nonPhenoConstrainedChargesNtoNN : Multiset (Charges ℤ) :=
 
   These trees can be found with e.g.
   `#eval nonPhenoConstrainedChargesExt nextToNearestNeighbor`. -/
-def nonPhenoConstrainedCharges : (I : CodimensionOneConfig) →  Multiset (Charges ℤ)
-  | same => nonPhenoConstrainedChargesSame
-  | nearestNeighbor => nonPhenoConstrainedChargesNN
-  | nextToNearestNeighbor => nonPhenoConstrainedChargesNtoNN
+def viableCharges : (I : CodimensionOneConfig) →  Multiset (Charges ℤ)
+  | same => viableChargesSame
+  | nearestNeighbor => viableChargesNN
+  | nextToNearestNeighbor => viableChargesNtoNN
 
 /-!
 
@@ -184,42 +400,42 @@ def nonPhenoConstrainedCharges : (I : CodimensionOneConfig) →  Multiset (Charg
 
 -/
 
-lemma nonPhenoConstrainedCharges_card (I : CodimensionOneConfig) :
-    (nonPhenoConstrainedCharges I).card =
+lemma viableCharges_card (I : CodimensionOneConfig) :
+    (viableCharges I).card =
     if I = .same then 102 else
     if I = .nearestNeighbor then 71 else 51  := by
   decide +revert
 
-lemma isComplete_of_mem_nonPhenoConstrainedCharge (I : CodimensionOneConfig) :
-    ∀ x ∈ (nonPhenoConstrainedCharges I), IsComplete x := by
+lemma isComplete_of_mem_viableCharges (I : CodimensionOneConfig) :
+    ∀ x ∈ (viableCharges I), IsComplete x := by
  revert I
  decide
 
-lemma allowsTerm_topYukawa_of_mem_nonPhenoConstrainedCharge (I : CodimensionOneConfig) :
-    ∀ x ∈ (nonPhenoConstrainedCharges I), x.AllowsTerm topYukawa := by
+lemma allowsTerm_topYukawa_of_mem_viableCharges (I : CodimensionOneConfig) :
+    ∀ x ∈ (viableCharges I), x.AllowsTerm topYukawa := by
   revert I
   decide
 
 set_option maxRecDepth 2000 in
-lemma not_isPhenoConstrained_of_mem_nonPhenoConstrainedCharges (I : CodimensionOneConfig) :
-    ∀ x ∈ (nonPhenoConstrainedCharges I), ¬ IsPhenoConstrained x := by
+lemma not_isPhenoConstrained_of_mem_viableCharges (I : CodimensionOneConfig) :
+    ∀ x ∈ (viableCharges I), ¬ IsPhenoConstrained x := by
   revert I
   decide
 
 set_option maxRecDepth 2000 in
-lemma not_yukawaGeneratesDangerousAtLevel_one_of_mem_nonPhenoConstrainedCharges
+lemma not_yukawaGeneratesDangerousAtLevel_one_of_mem_viableCharges
     (I : CodimensionOneConfig) :
-    ∀ x ∈ (nonPhenoConstrainedCharges I), ¬ YukawaGeneratesDangerousAtLevel x 1 := by
+    ∀ x ∈ (viableCharges I), ¬ YukawaGeneratesDangerousAtLevel x 1 := by
   revert I
   decide
 
-lemma card_five_bar_le_of_mem_nonPhenoConstrainedCharges (I : CodimensionOneConfig) :
-    ∀ x ∈ (nonPhenoConstrainedCharges I), x.2.2.1.card ≤ 2 := by
+lemma card_five_bar_le_of_mem_viableCharges (I : CodimensionOneConfig) :
+    ∀ x ∈ (viableCharges I), x.2.2.1.card ≤ 2 := by
   revert I
   decide
 
-lemma card_ten_le_of_mem_nonPhenoConstrainedCharges (I : CodimensionOneConfig) :
-    ∀ x ∈ (nonPhenoConstrainedCharges I), x.2.2.2.card ≤ 2 := by
+lemma card_ten_le_of_mem_viableCharges (I : CodimensionOneConfig) :
+    ∀ x ∈ (viableCharges I), x.2.2.2.card ≤ 2 := by
   revert I
   decide
 
@@ -227,12 +443,13 @@ lemma card_ten_le_of_mem_nonPhenoConstrainedCharges (I : CodimensionOneConfig) :
 
 ## Pheno insert
 -/
+
 set_option maxRecDepth 2000 in
-lemma phenoInsert_Q5_same  :
+lemma not_viable_of_insert_5_bar_viableCharges_same  :
     ∀ q5 ∈ same.allowedBarFiveCharges,
-    ∀ x ∈ (nonPhenoConstrainedCharges same),
+    ∀ x ∈ (viableCharges same),
     let y : Charges ℤ := (x.1, x.2.1, insert q5 x.2.2.1, x.2.2.2)
-    IsPhenoConstrained y ∨ y ∈ nonPhenoConstrainedCharges same
+    IsPhenoConstrained y ∨ y ∈ viableCharges same
     ∨  YukawaGeneratesDangerousAtLevel y 1 := by
   intro q5 hq5
   fin_cases hq5
@@ -245,11 +462,11 @@ lemma phenoInsert_Q5_same  :
   · decide
 
 set_option maxRecDepth 2000 in
-lemma phenoInsert_Q5_nn  :
+lemma not_viable_of_insert_5_bar_viableCharges_nn  :
     ∀ q5 ∈ nearestNeighbor.allowedBarFiveCharges,
-    ∀ x ∈ (nonPhenoConstrainedCharges nearestNeighbor),
+    ∀ x ∈ (viableCharges nearestNeighbor),
     let y : Charges ℤ := (x.1, x.2.1, insert q5 x.2.2.1, x.2.2.2)
-    IsPhenoConstrained y ∨ y ∈ nonPhenoConstrainedCharges nearestNeighbor
+    IsPhenoConstrained y ∨ y ∈ viableCharges nearestNeighbor
     ∨  YukawaGeneratesDangerousAtLevel y 1 := by
   intro q5 hq5
   fin_cases hq5
@@ -261,11 +478,11 @@ lemma phenoInsert_Q5_nn  :
   · decide
 
 set_option maxRecDepth 2000 in
-lemma phenoInsert_Q5_nnTon  :
+lemma not_viable_of_insert_5_bar_viableCharges_nnTon  :
     ∀ q5 ∈ nextToNearestNeighbor.allowedBarFiveCharges,
-    ∀ x ∈ (nonPhenoConstrainedCharges nextToNearestNeighbor),
+    ∀ x ∈ (viableCharges nextToNearestNeighbor),
     let y : Charges ℤ := (x.1, x.2.1, insert q5 x.2.2.1, x.2.2.2)
-    IsPhenoConstrained y ∨ y ∈ nonPhenoConstrainedCharges nextToNearestNeighbor
+    IsPhenoConstrained y ∨ y ∈ viableCharges nextToNearestNeighbor
     ∨ YukawaGeneratesDangerousAtLevel y 1 := by
   intro q5 hq5
   fin_cases hq5
@@ -276,11 +493,11 @@ lemma phenoInsert_Q5_nnTon  :
   · decide
   · decide
 
-lemma phenoInsert_Q5 (I : CodimensionOneConfig) :
+lemma not_viable_of_insert_5_bar_viableCharges (I : CodimensionOneConfig) :
     ∀ q5 ∈ I.allowedBarFiveCharges,
-    ∀ x ∈ (nonPhenoConstrainedCharges I),
+    ∀ x ∈ (viableCharges I),
     let y : Charges ℤ := (x.1, x.2.1, insert q5 x.2.2.1, x.2.2.2)
-    IsPhenoConstrained y ∨ y ∈ nonPhenoConstrainedCharges I
+    IsPhenoConstrained y ∨ y ∈ viableCharges I
     ∨  YukawaGeneratesDangerousAtLevel y 1 := by
   fin_cases I
   · exact phenoInsert_Q5_same
@@ -291,9 +508,9 @@ lemma phenoInsert_Q5 (I : CodimensionOneConfig) :
 set_option maxRecDepth 2000 in
 lemma phenoInsert_Q10_same  :
     ∀ q10 ∈ same.allowedTenCharges,
-    ∀ x ∈ (nonPhenoConstrainedCharges same),
+    ∀ x ∈ (viableCharges same),
     let y : Charges ℤ := (x.1, x.2.1, x.2.2.1, insert q10 x.2.2.2)
-    IsPhenoConstrained y ∨ y ∈ nonPhenoConstrainedCharges same
+    IsPhenoConstrained y ∨ y ∈ viableCharges same
     ∨  YukawaGeneratesDangerousAtLevel y 1 := by
   intro q5 hq5
   fin_cases hq5
@@ -308,9 +525,9 @@ lemma phenoInsert_Q10_same  :
 set_option maxRecDepth 2000 in
 lemma phenoInsert_Q10_nn  :
     ∀ q10 ∈ nearestNeighbor.allowedTenCharges,
-    ∀ x ∈ (nonPhenoConstrainedCharges nearestNeighbor),
+    ∀ x ∈ (viableCharges nearestNeighbor),
     let y : Charges ℤ := (x.1, x.2.1, x.2.2.1, insert q10 x.2.2.2)
-    IsPhenoConstrained y ∨ y ∈ nonPhenoConstrainedCharges nearestNeighbor
+    IsPhenoConstrained y ∨ y ∈ viableCharges nearestNeighbor
     ∨  YukawaGeneratesDangerousAtLevel y 1 := by
   intro q5 hq5
   fin_cases hq5
@@ -319,9 +536,9 @@ lemma phenoInsert_Q10_nn  :
 set_option maxRecDepth 2000 in
 lemma phenoInsert_Q10_nnTon  :
     ∀ q10 ∈ nextToNearestNeighbor.allowedTenCharges,
-    ∀ x ∈ (nonPhenoConstrainedCharges nextToNearestNeighbor),
+    ∀ x ∈ (viableCharges nextToNearestNeighbor),
     let y : Charges ℤ := (x.1, x.2.1, x.2.2.1, insert q10 x.2.2.2)
-    IsPhenoConstrained y ∨ y ∈ nonPhenoConstrainedCharges nextToNearestNeighbor
+    IsPhenoConstrained y ∨ y ∈ viableCharges nextToNearestNeighbor
     ∨  YukawaGeneratesDangerousAtLevel y 1 := by
   intro q5 hq5
   fin_cases hq5
@@ -329,14 +546,96 @@ lemma phenoInsert_Q10_nnTon  :
 
 lemma phenoInsert_Q10 (I : CodimensionOneConfig) :
     ∀ q10 ∈ I.allowedTenCharges,
-    ∀ x ∈ (nonPhenoConstrainedCharges I),
+    ∀ x ∈ (viableCharges I),
     let y : Charges ℤ := (x.1, x.2.1, x.2.2.1, insert q10 x.2.2.2)
-    IsPhenoConstrained y ∨ y ∈ nonPhenoConstrainedCharges I
+    IsPhenoConstrained y ∨ y ∈ viableCharges I
     ∨  YukawaGeneratesDangerousAtLevel y 1 := by
   fin_cases I
   · exact phenoInsert_Q10_same
   · exact phenoInsert_Q10_nn
   · exact phenoInsert_Q10_nnTon
+
+/-!
+
+## Proof of completeness.
+
+-/
+
+#eval
+    (((minimallyAllowsTermsOfFinset nextToNearestNeighbor.allowedBarFiveCharges
+        nextToNearestNeighbor.allowedTenCharges topYukawa).bind <|
+      completions nextToNearestNeighbor.allowedBarFiveCharges nextToNearestNeighbor.allowedTenCharges).dedup.filter
+    fun x => ¬ IsPhenoConstrained x ∧ ¬ YukawaGeneratesDangerousAtLevel x 1)
+
+
+
+set_option maxRecDepth 2000 in
+lemma completionTopYukawa_subset_nonPhenoConstrainedCharges :
+    ∀ x ∈ (completionTopYukawa I), x ∈ nonPhenoConstrainedCharges I := by
+  decide +revert
+
+set_option maxRecDepth 2000 in
+lemma not_isPhenoConstrained_mem_nonPhenoConstrainedCharges {x : Charges}
+    (hx : ¬ x.IsPhenoConstrained ∧ ¬ x.YukawaGeneratesDangerousAtLevel 1)
+    (hsub : x ∈ ofFinset I.allowedBarFiveCharges I.allowedTenCharges)
+    (hcomplete : IsComplete x) :
+    x ∉ nonPhenoConstrainedCharges I → ¬ ((¬ IsPhenoConstrained x ∧
+    ¬ YukawaGeneratesDangerousAtLevel x 1) ∧
+      AllowsTerm x topYukawa) := by
+  by_cases hn : ¬ (AllowsTerm x topYukawa)
+  · simp [hn]
+  rw [not_and]
+  simp only [hn, imp_false]
+  simp at hn
+  obtain ⟨y, y_mem, hyx⟩ :=
+    exists_subset_completionTopYukawa_of_not_isPhenoConstrained hx hn hsub hcomplete
+
+  refine subset_insert_filter_card_zero (nonPhenoConstrainedCharges I)
+    I.allowedBarFiveCharges I.allowedTenCharges (fun x =>
+      (¬x.IsPhenoConstrained ∧ ¬x.YukawaGeneratesDangerousAtLevel 1))
+    ?_ ?_ y ?_ x hyx hsub ?_ ?_
+  · intro x y hxy
+    simp only [Decidable.not_not]
+    simp
+    intro h1 h2
+    apply yukawaGeneratesDangerousAtLevel_of_subset hxy
+    apply h1
+    intro hn
+    apply h2
+    exact isPhenoConstrained_mono hxy hn
+  · intro x
+    exact fun a => isComplete_of_mem_nonPhenoConstrainedCharge I x a
+  · apply completionTopYukawa_subset_nonPhenoConstrainedCharges
+    exact y_mem
+  · intro q10
+    rw [Multiset.empty_eq_zero, Multiset.eq_zero_iff_forall_notMem]
+    simp
+    intro z hz hzP h2
+    have h1 := phenoInsert_Q10 I q10 q10.2 z hz
+    simp_all
+  · intro q5
+    rw [Multiset.empty_eq_zero, Multiset.eq_zero_iff_forall_notMem]
+    simp
+    intro z hz hzP h2
+    have h1 := phenoInsert_Q5 I q5 q5.2 z hz
+    simp_all
+
+lemma not_isPhenoConstrained_iff_mem_nonPhenoConstrainedCharge {x : Charges}
+    (hsub : x ∈ ofFinset I.allowedBarFiveCharges I.allowedTenCharges) :
+    AllowsTerm x topYukawa ∧
+    ¬ IsPhenoConstrained x ∧ ¬ YukawaGeneratesDangerousAtLevel x 1 ∧ IsComplete x ↔
+    x ∈ nonPhenoConstrainedCharges I := by
+  constructor
+  · intro ⟨hTop, hPheno, hY, hComplete⟩
+    by_contra hn
+    apply not_isPhenoConstrained_mem_nonPhenoConstrainedCharges ⟨hPheno, hY⟩ hsub hComplete hn
+    simp_all
+  · intro h
+    refine ⟨?_, ?_, ?_, ?_⟩
+    · exact allowsTerm_topYukawa_of_mem_nonPhenoConstrainedCharge I x h
+    · exact not_isPhenoConstrained_of_mem_nonPhenoConstrainedCharges I x h
+    · exact not_yukawaGeneratesDangerousAtLevel_one_of_mem_nonPhenoConstrainedCharges I x h
+    · exact isComplete_of_mem_nonPhenoConstrainedCharge I x h
 
 end Charges
 
